

Solved selected problems of Analytical Mechanics by Nivaldo Lemos

Franco Zacco

Solution. 1.1 Let

$$(x^2 + y^2)dx + xzdz = 0 \quad (x^2 + y^2)dy + yzdz = 0$$

be constraints.

- (a) We have two constraints that can be expressed as 1-forms $\omega^1 = 0$ and $\omega^2 = 0$ where

$$\omega^1 = (x^2 + y^2)dx + xzdz \quad \omega^2 = (x^2 + y^2)dy + yzdz$$

Also, $d\omega^1$ and $d\omega^2$ are

$$d\omega^1 = 2ydy \wedge dx + zdx \wedge dz \quad \text{and} \quad d\omega^2 = 2xdx \wedge dy + zdy \wedge dz$$

So, let us consider them separately, i.e. we want to compute $d\omega^1 \wedge \omega^1$ and $d\omega^2 \wedge \omega^2$ as follows

$$\begin{aligned} d\omega^1 \wedge \omega^1 &= (2ydy \wedge dx + zdx \wedge dz) \wedge ((x^2 + y^2)dx + xzdz) \\ &= 2xyz \, dy \wedge dx \wedge dz \end{aligned}$$

And

$$\begin{aligned} d\omega^2 \wedge \omega^2 &= (2xdx \wedge dy + zdy \wedge dz) \wedge ((x^2 + y^2)dy + yzdz) \\ &= 2xyz \, dx \wedge dy \wedge dz \end{aligned}$$

We see that $d\omega^1 \wedge \omega^1 \neq 0$ unless $x = y = z = 0$ and the same happens for $d\omega^2 \wedge \omega^2$.

Therefore, they are not integrable when considered separately.

- (b) The 2-form Ω defined by $\Omega = \omega^1 \wedge \omega^2$ is given by

$$\begin{aligned} \Omega &= (x^2 + y^2)dx + xzdz \wedge (x^2 + y^2)dy + yzdz \\ &= (x^2 + y^2)dx \wedge (x^2 + y^2)dy + (x^2 + y^2)dx \wedge yzdz \\ &\quad + xzdz \wedge (x^2 + y^2)dy \\ &= (x^2 + y^2)^2 dx \wedge dy + yz(x^2 + y^2)dx \wedge dz + xz(x^2 + y^2)dz \wedge dy \end{aligned}$$

It follows that

$$\begin{aligned}
d\omega^1 \wedge \Omega &= 2y(x^2 + y^2)^2 dy \wedge dx \wedge dx \wedge dy + 2y^2 z(x^2 + y^2) dy \wedge dx \wedge dx \wedge dz \\
&\quad + 2y x z(x^2 + y^2) dy \wedge dx \wedge dz \wedge dy + z(x^2 + y^2)^2 dx \wedge dz \wedge dy \wedge dx \\
&\quad + y z^2(x^2 + y^2) dx \wedge dz \wedge dx \wedge dz + x z^2(x^2 + y^2) dx \wedge dz \wedge dz \wedge dy \\
&= 0
\end{aligned}$$

And in the same way $d\omega^2 \wedge \Omega = 0$.

Therefore, the constraints are integrable when considered together.

On the other hand, let $x, y, z \neq 0$ then we see that

$$d \ln \frac{y}{x} = \frac{1}{y} dy - \frac{1}{x} dx$$

Also, let us consider the following

$$\begin{aligned}
y\omega^1 - x\omega^2 &= y(x^2 + y^2)dx + xyzdz - x(x^2 + y^2)dy - xyzdz \\
&= (x^2 + y^2)(ydx - xdy)
\end{aligned}$$

But since $\omega^1 = \omega^2 = 0$ then must be that

$$\begin{aligned}
ydx - xdy &= 0 \\
\frac{1}{y}dy - \frac{1}{x}dx &= 0
\end{aligned}$$

Then the constraints are equivalent to $d \ln(y/x) = 0$.

Now, considering the combination

$$\begin{aligned}
x\omega^1 + y\omega^2 &= x(x^2 + y^2)dx + x^2 z dz + y(x^2 + y^2)dy + y^2 z dz \\
&= (x^2 + y^2)(x dx + y dy + z dz)
\end{aligned}$$

Must be that $x dx + y dy + z dz = 0$ but we see that

$$d(x^2 + y^2 + z^2) = x dx + y dy + z dz$$

Therefore, the constraints are equivalent also to $xd(x^2 + y^2 + z^2) = 0$.

(c) Finally, integrating the equations

$$xd(x^2 + y^2 + z^2) = 0 \quad \text{and} \quad d \ln \frac{y}{x} = 0$$

We get that

$$\begin{aligned} \int d(x^2 + y^2 + z^2) &= 0 \\ x^2 + y^2 + z^2 + C'_1 &= 0 \\ x^2 + y^2 + z^2 &= C_1 \end{aligned}$$

And

$$\begin{aligned} \int d \ln \frac{y}{x} &= 0 \\ \ln \frac{y}{x} + C'_2 &= 0 \\ \frac{y}{x} &= 1 - e^{C'_2} \\ y &= C_2 x \end{aligned}$$

Where we renamed $C_1 = -C'_1$ and $C_2 = 1 - e^{C'_2}$.

□

Solution. 1.2 Let us consider the system from Example 1.18 in the case where $m_1 = m_2 = m_3 = m$ then the equations of motion become

$$\begin{aligned} m\ddot{x}_2 - \frac{k}{2}(x_3 - x_2 - l) &= 0 \\ m\ddot{x}_3 - mg + k(x_3 - x_2 - l) &= 0 \end{aligned}$$

Let us define $y = x_3 - x_2 - l$ then

$$\ddot{y} = \ddot{x}_3 - \ddot{x}_2$$

Then, subtracting the first equation from the second one we get that

$$\begin{aligned} m\ddot{x}_3 + k(x_3 - x_2 - l) - m\ddot{x}_2 + \frac{k}{2}(x_3 - x_2 - l) &= mg \\ (\ddot{x}_3 - \ddot{x}_2) + \frac{3k}{2m}(x_3 - x_2 - l) &= g \\ \ddot{y} + \frac{3k}{2m}y &= g \end{aligned}$$

We know that in terms of y the solution to this equation is

$$y(t) = C_1 \sin\left(\sqrt{\frac{3k}{2m}}t\right) + C_2 \cos\left(\sqrt{\frac{3k}{2m}}t\right) + \frac{2gm}{3k}$$

or letting $\omega = \sqrt{\frac{3k}{2m}}$ we get that

$$y(t) = C_1 \sin(\omega t) + C_2 \cos(\omega t) + \frac{2mg}{3k}$$

Using the initial conditions $x_2 = 0$ and $x_3 = l$ we can determine C_2 . We see that $y(t = 0) = l - 0 - l = 0$ then $C_2 = -\frac{2mg}{3k}$.

On the other hand,

$$\dot{y}(t) = C_1 \omega \cos(\omega t) - C_2 \omega \sin(\omega t)$$

And since the system starts from rest i.e. $\dot{y} = 0$ we get that $C_1 = 0$. Therefore the equation becomes

$$y(t) = \frac{2mg}{3k}(1 - \cos(\omega t)) = x_3 - x_2 - l$$

So, replacing in the first original differential equation we get that

$$\ddot{x}_2 + \frac{g}{3}(\cos(\omega t) - 1) = 0$$

Integrating with respect to t gives us

$$\dot{x}_2 = -\frac{g}{3} \int (\cos(\omega t) - 1) dt = \frac{g}{3\omega} \left[\omega t - \sin(\omega t) \right] + C$$

Where $C = 0$ since $\dot{x}_2 = 0$ at $t = 0$. Integrating again

$$\begin{aligned} x_2 &= \frac{g}{3} \int \left[-\frac{1}{\omega} \sin(\omega t) + t \right] dt \\ &= \frac{g}{3} \frac{\cos(\omega t)}{\omega^2} + \frac{g}{6} t^2 + C \\ &= \frac{2mg}{9k} \cos(\omega t) + \frac{g}{6} t^2 + C \end{aligned}$$

Where we replaced the value of ω . Now since $x_2 = 0$ when $t = 0$ we have that $C = -2mg/9k$, so, finally

$$x_2 = \frac{2mg}{9k} (\cos(\omega t) - 1) + \frac{g}{6} t^2$$

From the equation we got for \dot{x}_2 , let $t = \pi/2\omega$, at this moment $\sin(\omega t) = 1$ which is as negative as $-\sin(\omega t)$ can get. Hence

$$\omega t - \sin(\omega t) = \frac{\pi}{2} - 1$$

But since $\pi/2 > 1$, then, $\dot{x}_2 > 0$ at this moment. For any point later, t will grow even more and hence $\omega t - \sin(\omega t)$ will be positive.

Therefore if $t > 0$ then $\dot{x}_2 > 0$. □

Solution. 1.5 Let us consider Atwood's machine shown in Fig. 1.10. The string connecting M and m must be inextensible, so, let x be the vertical coordinate which determines the position of M , then must be that $x+c+r = l$ where l is the constant length of the string and c is the length between pulleys.

The kinetic energy experienced by M is then $T_M = M\dot{x}^2/2 = M\dot{r}^2/2$.

So the kinetic energy of the system is

$$T = \frac{M}{2}\dot{r}^2 + \frac{m}{2}(\dot{r}^2 + r^2\dot{\theta}^2) = \frac{m+M}{2}\dot{r}^2 + \frac{m}{2}r^2\dot{\theta}^2$$

On the other hand, for the potential energy since the string is inextensible then any change in the r coordinate will imply a change in potential energy for the M mass so we can write that

$$V = Mgr - mgr \cos \theta = gr(M - m \cos \theta)$$

Therefore, the Lagrangian is

$$L = T - V = \frac{m+M}{2}\dot{r}^2 + \frac{m}{2}r^2\dot{\theta}^2 - gr(M - m \cos \theta)$$

Now, we want to write Lagrange's equations for the system. We compute first the derivatives

$$\begin{aligned} \frac{\partial L}{\partial \dot{r}} &= (m+M)\dot{r} & \frac{\partial L}{\partial r} &= mr\dot{\theta}^2 - g(M - m \cos \theta) \\ \frac{\partial L}{\partial \dot{\theta}} &= mr^2\dot{\theta} & \frac{\partial L}{\partial \theta} &= -mgr \sin \theta \end{aligned}$$

Then the Lagrange's equations are

$$\begin{aligned} \frac{d}{dt} \left(\frac{\partial L}{\partial \dot{r}} \right) - \frac{\partial L}{\partial r} &= (m+M)\ddot{r} - mr\dot{\theta}^2 + g(M - m \cos \theta) = 0 \\ \frac{d}{dt} \left(\frac{\partial L}{\partial \dot{\theta}} \right) - \frac{\partial L}{\partial \theta} &= mr(2\dot{\theta}\dot{r} + r\ddot{\theta}) + mgr \sin \theta = 0 \end{aligned}$$

□

Solution. 1.6 Let us consider Huygens' cycloidal pendulum with the following parametric equations

$$x = R(\theta - \sin \theta) \quad y = R(1 - \cos \theta)$$

where the vertical y -axis points downward.

Then the kinetic energy of the system is given by

$$\begin{aligned} T &= \frac{m}{2}(\dot{x}^2 + \dot{y}^2) \\ &= \frac{m}{2}R^2[(\dot{\theta} - \dot{\theta} \cos \theta)^2 + \dot{\theta}^2 \sin^2 \theta] \\ &= \frac{m}{2}R^2[\dot{\theta}^2 - 2\dot{\theta}^2 \cos \theta + \dot{\theta}^2 \cos^2 \theta + \dot{\theta}^2 \sin^2 \theta] \\ &= \frac{m}{2}R^2[1 - 2\cos \theta + 1]\dot{\theta}^2 \\ &= 2mR^2 \left[\frac{1 - \cos \theta}{2} \right] \dot{\theta}^2 \\ &= 2mR^2 \sin^2 \left(\frac{\theta}{2} \right) \dot{\theta}^2 \end{aligned}$$

Where we used the trigonometric identity $\sin^2(\theta/2) = (1 - \cos \theta)/2$.

On the other hand, the potential energy only depends on y and since the y -axis points downward we have that

$$V = -mgy = -mgR(1 - \cos \theta)$$

Therefore, the Lagrangian of the system is

$$L = T - V = 2mR^2 \sin^2 \left(\frac{\theta}{2} \right) \dot{\theta}^2 + mgR(1 - \cos \theta)$$

Let now, $u = \cos(\theta/2)$ then $\theta = 2 \arccos(u)$, so the Lagrangian in terms of u is given by

$$\begin{aligned} L &= 2mR^2 \sin^2(\arccos(u)) \left(-\frac{2\dot{u}}{\sqrt{1-u^2}} \right)^2 + mgR(1 - \cos(2 \arccos(u))) \\ L &= 2mR^2(1 - u^2) \left(\frac{4\dot{u}^2}{1 - u^2} \right) + mgR(1 - 2\cos^2(\arccos(u)) + 1) \\ L &= 8mR^2\dot{u}^2 + 2mgR(1 - u^2) \end{aligned}$$

Then the Lagrange equation in terms of u is

$$\frac{d}{dt} \left(\frac{\partial L}{\partial \dot{u}} \right) - \frac{\partial L}{\partial u} = 16mR^2\ddot{u} + 4mgRu = 0$$

Finally, we can write this equation as

$$\begin{aligned} 4R^2\ddot{u} + gRu &= 0 \\ \ddot{u} &= -\frac{g}{4R}u \end{aligned}$$

This is the equation of a simple harmonic oscillator where $\omega^2 = g/4R$, or in terms of the period of oscillation $\omega = 2\pi/T$ then we get that

$$\begin{aligned}\frac{4\pi^2}{T^2} &= \frac{g}{4R} \\ T^2 &= \frac{16\pi^2 R}{g} \\ T &= 4\pi\sqrt{\frac{R}{g}}\end{aligned}$$

□

Solution. 1.7 Let a projectile fired near the surface of the earth. Taking the Cartesian coordinates as the generalized coordinates we have that the kinetic energy is

$$T = \frac{1}{2}mv^2 = \frac{1}{2}m(v_x^2 + v_y^2)$$

And the potential energy is

$$V = mgy$$

Therefore the lagrangian is given by

$$L = T - V = \frac{1}{2}m(v_x^2 + v_y^2) - mgy$$

We solve then Lagrange's equation to get the equations of motion as follows

$$\begin{aligned}\frac{d}{dt}\left(\frac{\partial L}{\partial v_x}\right) - \frac{\partial L}{\partial x} + \frac{\partial \mathcal{F}}{\partial v_x} &= m\dot{v}_x + \lambda v_x = 0 \\ \frac{d}{dt}\left(\frac{\partial L}{\partial v_y}\right) - \frac{\partial L}{\partial y} + \frac{\partial \mathcal{F}}{\partial v_y} &= m\dot{v}_y + mg + \lambda v_y = 0\end{aligned}$$

Then the equations of motion are

$$\ddot{x} + \frac{\lambda}{m}\dot{x} = 0 \quad \ddot{y} + \frac{\lambda}{m}\dot{y} = -g$$

□

Solution. 1.8

(a) Let us define the following lagrangian

$$L = e^{\lambda t/m} \left[\frac{m}{2} (\dot{x}^2 + \dot{y}^2) - mgy \right]$$

Lagrange's equation for the x coordinate is

$$\begin{aligned} \frac{d}{dt} \left(\frac{\partial L}{\partial \dot{x}} \right) - \frac{\partial L}{\partial x} &= 0 \\ \frac{d}{dt} \left(e^{\lambda t/m} m \dot{x} \right) &= 0 \\ m e^{\lambda t/m} \ddot{x} + \lambda e^{\lambda t/m} \dot{x} &= 0 \\ \ddot{x} + \frac{\lambda}{m} \dot{x} &= 0 \end{aligned}$$

And Lagrange's equation for the y coordinate is

$$\begin{aligned} \frac{d}{dt} \left(\frac{\partial L}{\partial \dot{y}} \right) - \frac{\partial L}{\partial y} &= 0 \\ \frac{d}{dt} \left(e^{\lambda t/m} m \dot{y} \right) + m g e^{\lambda t/m} &= 0 \\ m e^{\lambda t/m} \ddot{y} + \lambda e^{\lambda t/m} \dot{y} + m g e^{\lambda t/m} &= 0 \\ \ddot{y} + \frac{\lambda}{m} \dot{y} &= -g \end{aligned}$$

(b) Let us solve the equations of motion now assuming the projectile is fired from the origin with a velocity of magnitude v_0 making an angle θ_0 with the horizontal.

We see that the equation for x can be solved by integration, first let us rename $v = \dot{x}$ then the equation becomes

$$\begin{aligned} \frac{dv}{dt} &= -\frac{\lambda}{m} v \\ \int \frac{dv}{v} &= -\frac{\lambda}{m} \int dt \\ \log(v) &= -\frac{\lambda}{m} t + C \\ v &= c_1 e^{-\lambda t/m} \end{aligned}$$

Now, replacing back again v and integrating again we get that

$$\begin{aligned} \int dx &= c_1 \int e^{-\lambda t/m} dt \\ x &= -c_1 \frac{m}{\lambda} e^{-\lambda t/m} + c_2 \end{aligned}$$

We can determine the values of c_1 and c_2 by plugging in the initial conditions. We know that $x(t=0) = 0$ hence $0 = c_2 - c_1 m/\lambda$.

Also, we know that $\dot{x}(t=0) = v_0 \cos \theta_0$ so since $\dot{x} = c_1 e^{-\lambda t/m}$ we get that $c_1 = v_0 \cos \theta_0$, and using this result we get that $c_2 = v_0 m \cos \theta_0 / \lambda$. Then the equation for x becomes

$$x = \frac{v_0 \cos \theta_0 m}{\lambda} (1 - e^{-\lambda t/m})$$

On the other hand, to solve the equation for y first we solve the homogeneous equation $\ddot{y} + \lambda \dot{y}/m = 0$ and then we add a particular solution to get the general solution. The homogeneous equation has the same form as the one we solved for x so the solution is

$$y = c_2 - c_1 \frac{m}{\lambda} e^{-\lambda t/m}$$

Now, let us try the particular solution $y = -(mg/\lambda)t$ then we see that $\dot{y} = -mg/\lambda$ and $\ddot{y} = 0$ so we get that

$$0 + \frac{\lambda}{m} \left(-\frac{mg}{\lambda} \right) = -g$$

So $y = -(mg/\lambda)t$ is a particular solution. Then the general solution is

$$y = c_2 - c_1 \frac{m}{\lambda} e^{-\lambda t/m} - \frac{mg}{\lambda} t$$

When $t = 0$ we get that $y(t=0) = 0$ then $c_2 = c_1 m / \lambda$. Also, we have that $\dot{y} = c_1 e^{-\lambda t/m} - mg/\lambda$ and when $t = 0$ we know that $\dot{y} = v_0 \sin \theta_0$ so $c_1 = v_0 \sin \theta_0 + mg/\lambda$ and hence $c_2 = v_0 \sin \theta_0 m / \lambda + m^2 g / \lambda^2$. Therefore the general solution becomes

$$y = \left(v_0 \sin \theta_0 \frac{m}{\lambda} + \frac{m^2 g}{\lambda^2} \right) (1 - e^{-\lambda t/m}) - \frac{mg}{\lambda} t$$

(c) From the equation for x we can get the time t as follows

$$\begin{aligned} 1 - e^{-\lambda t/m} &= \frac{\lambda x}{m v_0 \cos \theta_0} \\ -\frac{\lambda t}{m} &= \log \left(1 - \frac{\lambda x}{m v_0 \cos \theta_0} \right) \\ t &= -\frac{m}{\lambda} \log \left(1 - \frac{\lambda x}{m v_0 \cos \theta_0} \right) \end{aligned}$$

Now, replacing t in the equation for y we get the equation for the trajectory of the projectile

$$\begin{aligned} y &= \left(v_0 \sin \theta_0 \frac{m}{\lambda} + \frac{m^2 g}{\lambda^2} \right) \frac{\lambda x}{m v_0 \cos \theta_0} + \frac{m^2 g}{\lambda^2} \log \left(1 - \frac{\lambda x}{m v_0 \cos \theta_0} \right) \\ y &= \left(\tan \theta_0 + \frac{mg}{\lambda v_0 \cos \theta_0} \right) x + \frac{m^2 g}{\lambda^2} \log \left(1 - \frac{\lambda x}{m v_0 \cos \theta_0} \right) \end{aligned}$$

□

Solution. 1.9

- (a) Taking the generalized coordinate x from the middle point when both springs are at its natural length and θ measured from vertical then the coordinates of the mass m are

$$\begin{aligned}x' &= x + l \sin \theta \\y' &= l \cos \theta\end{aligned}$$

So the velocities of m are

$$\begin{aligned}\dot{x}' &= \dot{x} + \dot{\theta}l \cos \theta \\ \dot{y}' &= -\dot{\theta}l \sin \theta\end{aligned}$$

Then the kinetic energy is

$$\begin{aligned}T &= \frac{1}{2}m((\dot{x} + \dot{\theta}l \cos \theta)^2 + (-\dot{\theta}l \sin \theta)^2) \\ &= \frac{1}{2}m(\dot{x}^2 + 2\dot{x}\dot{\theta}l \cos \theta + \dot{\theta}^2l^2 \cos^2 \theta + \dot{\theta}^2l^2 \sin^2 \theta) \\ &= \frac{1}{2}m(\dot{x}^2 + 2\dot{x}\dot{\theta}l \cos \theta + \dot{\theta}^2l^2)\end{aligned}$$

And the potential energy is

$$V = -mgl \cos \theta + \frac{1}{2}k(x^2 + x^2) = -mgl \cos \theta + kx^2$$

Where we assumed that the natural length of the springs is 0 for simplicity.

Then the Lagrangian is given by

$$L = T - V = \frac{1}{2}m(\dot{x}^2 + 2\dot{x}\dot{\theta}l \cos \theta + \dot{\theta}^2l^2) + mgl \cos \theta - kx^2$$

Now, we solve the Lagrange's equation as follows

$$\begin{aligned}\frac{d}{dt} \left(\frac{\partial L}{\partial \dot{x}} \right) - \frac{\partial L}{\partial x} &= 0 \\ \frac{d}{dt} \left(m(\dot{x} + \dot{\theta}l \cos \theta) \right) + 2kx &= 0 \\ m(\ddot{x} + \ddot{\theta}l \cos \theta - \dot{\theta}^2l \sin \theta) + 2kx &= 0\end{aligned}$$

And

$$\begin{aligned}\frac{d}{dt} \left(\frac{\partial L}{\partial \dot{\theta}} \right) - \frac{\partial L}{\partial \theta} &= 0 \\ \frac{d}{dt} \left(m(\dot{x}l \cos \theta + \dot{\theta}l^2) \right) + m\dot{x}\dot{\theta}l \sin \theta + mgl \sin \theta &= 0 \\ m(\ddot{x}l \cos \theta - \dot{x}\dot{\theta}l \sin \theta + \ddot{\theta}l^2) + m\dot{x}\dot{\theta}l \sin \theta + mgl \sin \theta &= 0 \\ m(\ddot{x}l \cos \theta + \ddot{\theta}l^2) + mgl \sin \theta &= 0\end{aligned}$$

- (b) In the case of small angular oscillations $\sin \theta \approx \theta$ and $\cos \theta \approx 1$ and terms such as θ^n and $\dot{\theta}^n$ can be neglected. Then the equations of motion become

$$\begin{aligned} m(\ddot{x} + \ddot{\theta}l) + 2kx &= 0 \\ m(\ddot{x} + \ddot{\theta}l) + mg\theta &= 0 \end{aligned}$$

Then subtracting both equations we see that

$$\begin{aligned} 2kx - mg\theta &= 0 \\ x &= \frac{mg}{2k}\theta \end{aligned}$$

So x can be written as $x = \alpha\theta$ where $\alpha = mg/2k$.

Now, computing $\ddot{x} = \alpha\ddot{\theta}$ and replacing it in the second approximated equation of motion gives us

$$\begin{aligned} m(\alpha\ddot{\theta} + \ddot{\theta}l) + mg\theta &= 0 \\ \ddot{\theta}(l + \alpha) + g\theta &= 0 \\ \ddot{\theta} + \frac{g}{l'}\theta &= 0 \end{aligned}$$

We see that the last equation is the differential equation which governs a small oscillation pendulum of length l' where l' is

$$l' = l + \frac{mg}{2k}$$

□

Solution. 1.10 Let the force between two charged particles in motion be

$$F = \frac{ee'}{r^2} \left[1 + \frac{r\ddot{r}}{c^2} - \frac{\dot{r}^2}{2c^2} \right] = ee' \left[\frac{1}{r^2} + \frac{\ddot{r}}{rc^2} - \frac{\dot{r}^2}{2r^2c^2} \right]$$

Let us define the generalised potential as follows

$$U = ee' \left[\frac{1}{r} + \frac{\dot{r}^2}{2rc^2} \right]$$

Then we see that F can be written as

$$\begin{aligned} F &= -\frac{\partial U}{\partial r} + \frac{d}{dt} \left(\frac{\partial U}{\partial \dot{r}} \right) \\ &= ee' \left[\left(\frac{1}{r^2} + \frac{\dot{r}^2}{2r^2c^2} \right) + \left(\frac{\ddot{r}}{rc^2} - \frac{\dot{r}^2}{r^2c^2} \right) \right] \\ &= ee' \left[\frac{1}{r^2} + \frac{\ddot{r}}{rc^2} - \frac{\dot{r}^2}{2r^2c^2} \right] \end{aligned}$$

So U is the generalised potential associated to F .

Now, if a charge is in the presence of another charge held fixed at the origin, then the force F is the force between them, but r is the polar radial coordinate of the free charge. Then the kinetic energy of the system is

$$T = \frac{m}{2} (\dot{r}^2 + r^2 \dot{\theta}^2)$$

Where m is the mass of the charge. Then the Lagrangian of the system is

$$L = T - U = \frac{m}{2} (\dot{r}^2 + r^2 \dot{\theta}^2) - ee' \left[\frac{1}{r} + \frac{\dot{r}^2}{2rc^2} \right]$$

Therefore the Lagrange's equations are

$$\begin{aligned} \frac{d}{dt} \left(\frac{\partial L}{\partial \dot{r}} \right) - \frac{\partial L}{\partial r} &= 0 \\ \frac{d}{dt} \left(m\dot{r} - \frac{ee'\dot{r}}{rc^2} \right) - \left[mr\dot{\theta}^2 + ee' \left[\frac{1}{r^2} + \frac{\dot{r}^2}{2r^2c^2} \right] \right] &= 0 \\ m\ddot{r} - ee' \left[\frac{\ddot{r}}{rc^2} - \frac{\dot{r}^2}{r^2c^2} \right] - \left[mr\dot{\theta}^2 + ee' \left[\frac{1}{r^2} + \frac{\dot{r}^2}{2r^2c^2} \right] \right] &= 0 \\ m(\ddot{r} - r\dot{\theta}^2) - ee' \left[\frac{1}{r^2} + \frac{\ddot{r}}{rc^2} - \frac{\dot{r}^2}{2r^2c^2} \right] &= 0 \end{aligned}$$

And

$$\begin{aligned} \frac{d}{dt} \left(\frac{\partial L}{\partial \dot{\theta}} \right) - \frac{\partial L}{\partial \theta} &= 0 \\ mr^2\dot{\theta} &= 0 \end{aligned}$$

But, we see from the last equation that $\dot{\theta} = 0$ then the first equation of motion becomes

$$m\ddot{r} = ee' \left[\frac{1}{r^2} + \frac{\ddot{r}}{rc^2} - \frac{\dot{r}^2}{2r^2c^2} \right]$$

□

Solution. 1.16 Let Bateman's Lagrangian

$$L = e^{\lambda t} \left(\frac{m}{2} \dot{x}^2 - \frac{m\omega^2}{2} x^2 \right)$$

Then Lagrange's equation for this Lagrangian is

$$\begin{aligned} \frac{d}{dt} \left(\frac{\partial L}{\partial \dot{x}} \right) - \frac{\partial L}{\partial x} &= 0 \\ \frac{d}{dt} (e^{\lambda t} m \dot{x}) - e^{\lambda t} m \omega^2 x &= 0 \\ \lambda e^{\lambda t} m \dot{x} + e^{\lambda t} m \ddot{x} - e^{\lambda t} m \omega^2 x &= 0 \\ \ddot{x} + \lambda \dot{x} - \omega^2 x &= 0 \end{aligned}$$

We see that this is the equation of motion of a damped harmonic oscillator. Let us define $q = e^{\lambda t/2} x$ then we see that $q^2 = e^{\lambda t} x^2$, also, from the derivative of q with respect to time we see that

$$\begin{aligned} \dot{q} &= \frac{\lambda}{2} e^{\lambda t/2} x + e^{\lambda t/2} \dot{x} \\ e^{\lambda t/2} \dot{x} &= \dot{q} - \frac{\lambda}{2} e^{\lambda t/2} x \\ e^{\lambda t/2} \dot{x} &= \dot{q} - \frac{\lambda}{2} q \\ e^{\lambda t} \dot{x}^2 &= \left(\dot{q} - \frac{\lambda}{2} q \right)^2 \end{aligned}$$

Then the Lagrangian L becomes

$$L = e^{\lambda t} \frac{m}{2} \dot{x}^2 - e^{\lambda t} \frac{m\omega^2}{2} x^2 = \frac{m}{2} \left(\dot{q} - \frac{\lambda}{2} q \right)^2 - \frac{m\omega^2}{2} q^2$$

Hence the Lagrangian doesn't have an explicit time dependence. □

Solution. 1.18

- (a) Let us consider Atwood's machine in terms of $x = x_1$ with a massive pulley and a massive string with uniform linear mass density λ . The kinetic energy of the system is then given by

$$T = \frac{1}{2}(m_1 + m_2 + m_s)\dot{x}^2 + \frac{1}{2}I\omega^2$$

Where the first term takes into account the masses m_1 , m_2 and the mass of the string m_s . The second term is the rotational kinetic energy because of the massive pulley, but we know that $\omega = \dot{x}/R$ where R is the radius of the pulley, then

$$T = \frac{1}{2}(m_1 + m_2 + m_s + I/R^2)\dot{x}^2$$

On the other hand, the potential energy because of the masses m_1 and m_2 is $-m_1gx + m_2gx$ since when one mass goes up the other goes down by the same amount.

Now, for the string, let l be the length of the hanging part of the string, then the mass of the string on the left side is $\lambda x_1 = \lambda x$ and the mass on the right side is then $\lambda(l - x)$. Taking into account the displacements of the centers of mass of each side we get that the total potential energy is

$$\begin{aligned} V &= -m_1gx + m_2gx - \lambda xg\frac{x}{2} - \lambda(l - x)g\frac{(l - x)}{2} \\ &= (m_2 - m_1)gx - \frac{\lambda g}{2}x^2 - \frac{\lambda g}{2}(l - x)^2 \end{aligned}$$

Therefore the Lagrangian of the system is

$$L = \frac{1}{2}(m_1 + m_2 + m_s + I/R^2)\dot{x}^2 + (m_1 - m_2)gx + \frac{\lambda g}{2}x^2 + \frac{\lambda g}{2}(l - x)^2$$

- (b) Lagrange's equation for x is then

$$\begin{aligned} \frac{d}{dt}\left(\frac{\partial L}{\partial \dot{x}}\right) - \frac{\partial L}{\partial x} &= 0 \\ \frac{d}{dt}((m_1 + m_2 + m_s + I/R^2)\dot{x}) - (m_1 - m_2)g - \lambda gx + \lambda g(l - x) &= 0 \\ (m_1 + m_2 + m_s + I/R^2)\ddot{x} - (m_1 - m_2)g - \lambda gx + \lambda g(l - x) &= 0 \end{aligned}$$

- (c) Let $m_1 = m_2 = 0$ then the equation of motion becomes

$$\begin{aligned} (m_s + I/R^2)\ddot{x} - \lambda gx + \lambda g(l - x) &= 0 \\ (m_s + I/R^2)\ddot{x} - 2\lambda gx + \lambda gl &= 0 \\ \ddot{x} - b^2x + \frac{b^2l}{2} &= 0 \end{aligned}$$

Where $b = \sqrt{2\lambda g/(m_s + I/R^2)}$. We know that the solution to this differential equation is

$$x(t) = c_1 e^{bt} + c_2 e^{-bt} + \frac{l}{2}$$

From the initial conditions $x(0) = x_0$ and $\dot{x}(0) = 0$ we can determine c_1 and c_2 , so we get that

$$c_1 + c_2 = x_0 - \frac{l}{2}$$

And from $\dot{x}(t) = c_1 b e^{bt} - c_2 b e^{-bt}$ we get that $0 = c_1 - c_2$ so

$$c_1 = c_2 = \frac{1}{2} \left(x_0 - \frac{l}{2} \right)$$

Therefore

$$\begin{aligned} x(t) &= \frac{1}{2} \left(x_0 - \frac{l}{2} \right) (e^{bt} + e^{-bt}) + \frac{l}{2} \\ &= \left(x_0 - \frac{l}{2} \right) \frac{e^{bt} + e^{-bt}}{2} + \frac{l}{2} \\ &= \left(x_0 - \frac{l}{2} \right) \cosh bt + \frac{l}{2} \end{aligned}$$

If $x_0 = l/2$ we get that $x(t) = l/2$ which is the right physically expected solution since each half of the string is hanging statically on each side of the pulley.

- (d) The exponential behaviour of the speed of the string for t larger than a few time constants is physically correct since we are considering the case $m_1 = m_2 = 0$, so the string would slip and fall off the pulley increasing its velocity infinitely.

□

Solution. 1.19 Let the following lagrangian

$$L = \frac{1}{2} \frac{1}{1 + \lambda x^2} \left(\dot{x}^2 - \omega_0^2 x^2 \right) \quad \text{with} \quad \lambda > 0$$

(a) Then Lagrange's equation for x is

$$\begin{aligned} \frac{d}{dt} \left(\frac{\partial L}{\partial \dot{x}} \right) - \frac{\partial L}{\partial x} &= 0 \\ \frac{d}{dt} \left(\frac{\dot{x}}{1 + \lambda x^2} \right) - \frac{1}{2} \left(- \frac{2\lambda x}{(1 + \lambda x^2)^2} (\dot{x}^2 - \omega_0^2 x^2) - \frac{2\omega_0^2 x}{1 + \lambda x^2} \right) &= 0 \\ \left(\frac{\ddot{x}}{1 + \lambda x^2} - \frac{2\lambda x \dot{x}^2}{(1 + \lambda x^2)^2} \right) + \left(\frac{\lambda x}{(1 + \lambda x^2)^2} (\dot{x}^2 - \omega_0^2 x^2) + \frac{\omega_0^2 x}{1 + \lambda x^2} \right) &= 0 \\ \left(\frac{\ddot{x}(1 + \lambda x^2) - 2\lambda x \dot{x}^2}{(1 + \lambda x^2)^2} \right) + \frac{\lambda x \dot{x}^2 - \omega_0^2 \lambda x x^2 + \omega_0^2 x (1 + \lambda x^2)}{(1 + \lambda x^2)^2} &= 0 \\ \ddot{x}(1 + \lambda x^2) - 2\lambda x \dot{x}^2 + \lambda x \dot{x}^2 - \omega_0^2 \lambda x x^2 + \omega_0^2 x (1 + \lambda x^2) &= 0 \\ \ddot{x}(1 + \lambda x^2) - \lambda x \dot{x}^2 + \omega_0^2 x &= 0 \end{aligned}$$

(b) Let

$$x = A \sin(\omega t + \delta)$$

Then

$$\dot{x} = A\omega \cos(\omega t + \delta) \quad \text{and} \quad \ddot{x} = -A\omega^2 \sin(\omega t + \delta)$$

So replacing in the equation of motion we got from part (a) we see that

$$\begin{aligned} \ddot{x}(1 + \lambda x^2) - \lambda x \dot{x}^2 + \omega_0^2 x &= 0 \\ -A\omega^2 \sin(\omega t + \delta)(1 + \lambda A^2 \sin^2(\omega t + \delta)) - \lambda A \sin(\omega t + \delta) A^2 \omega^2 \cos^2(\omega t + \delta) \\ &+ \omega_0^2 A \sin(\omega t + \delta) = 0 \\ -A\omega^2 \sin(\omega t + \delta) - \lambda A^3 \omega^2 \sin^3(\omega t + \delta) - \lambda A^3 \omega^2 \sin(\omega t + \delta) \cos^2(\omega t + \delta) \\ &+ \omega_0^2 A \sin(\omega t + \delta) = 0 \end{aligned}$$

We see that if $t = n\pi/\omega - \delta$ for $n = 0, 1, \dots$ the equation is satisfied, so let us assume $t \neq n\pi/\omega - \delta$ and hence $\sin(\omega t + \delta) \neq 0$ then dividing by $\sin(\omega t + \delta)$ we get that

$$\begin{aligned} -A\omega^2 - \lambda A^3 \omega^2 \sin^2(\omega t + \delta) - \lambda A^3 \omega^2 \cos^2(\omega t + \delta) + \omega_0^2 A &= 0 \\ -A\omega^2 - \lambda A^3 \omega^2 (\sin^2(\omega t + \delta) + \cos^2(\omega t + \delta)) + \omega_0^2 A &= 0 \\ \omega^2 + \lambda A^2 \omega^2 - \omega_0^2 &= 0 \end{aligned}$$

So we see that this equation is satisfied if $\omega^2 + \lambda A^2 \omega^2 = \omega_0^2$. Therefore ω^2 must have the following value

$$\omega^2 = \frac{\omega_0^2}{1 + \lambda A^2}$$

□

Solution. 1.20 From equation (1.162) and taking $V(r) = -\kappa/r$ we get that

$$E = \frac{m}{2} \left(\frac{dr}{dt} \right)^2 + \frac{l^2}{2mr^2} - \frac{\kappa}{r}$$

So

$$\begin{aligned} \frac{m}{2} \left(\frac{dr}{dt} \right)^2 &= E + \frac{\kappa}{r} - \frac{l^2}{2mr^2} \\ \frac{dr}{dt} &= \sqrt{\frac{2}{m}} \sqrt{E + \frac{\kappa}{r} - \frac{l^2}{2mr^2}} \end{aligned}$$

Now, we integrate from $t = 0$ where $r = r_{min}$ (since the planet is at the perihelion) to t and r

$$\int_0^t dt = \sqrt{\frac{m}{2}} \int_{r_{min}}^r \frac{dr}{\sqrt{E + \frac{\kappa}{r} - \frac{l^2}{2mr^2}}}$$

Also, we see that

$$\begin{aligned} t &= \sqrt{\frac{m}{2}} \int_{r_{min}}^r \frac{dr}{\sqrt{\frac{\kappa}{r^2} \left(\frac{Er^2}{\kappa} + r - \frac{l^2}{2m\kappa} \right)}} \\ &= \sqrt{\frac{m}{2\kappa}} \int_{r_{min}}^r \frac{r dr}{\sqrt{\frac{Er^2}{\kappa} + r - \frac{l^2}{2m\kappa}}} \\ &= \sqrt{\frac{m}{2\kappa}} \int_{r_{min}}^r \frac{r dr}{\sqrt{\frac{Er^2}{\kappa} + r - \frac{p}{2}}} \end{aligned}$$

Where $p = l^2/m\kappa$. We know as well that $e = \sqrt{1 + 2El^2/m\kappa^2}$ so

$$-\frac{m}{2l^2}(1 - e^2) = \frac{E}{\kappa^2}$$

But also since $a = p(1 - e^2)^{-1}$ we get that

$$\frac{E}{\kappa} = -\frac{m\kappa}{2l^2}(1 - e^2) = -\frac{1}{2p}(1 - e^2) = -\frac{1}{2a}$$

then

$$t = \sqrt{\frac{m}{2\kappa}} \int_{r_{min}}^r \frac{r dr}{\sqrt{r - \frac{r^2}{2a} - \frac{a(1-e^2)}{2}}}$$

Where we also used that $p = a(1 - e^2)$.

Now, let us define ψ as $r = a(1 - e \cos \psi)$ so $dr = ea \sin \psi d\psi$. Then, replacing

in the integral we get that

$$\begin{aligned}
t &= \sqrt{\frac{m}{2\kappa}} \int_0^\psi \frac{ea^2(1 - e \cos \psi) \sin \psi d\psi}{\sqrt{a(1 - e \cos \psi) - \frac{a(1 - e \cos \psi)^2}{2} - \frac{a(1 - e^2)}{2}}} \\
&= \sqrt{\frac{m}{2\kappa}} \int_0^\psi \frac{e\sqrt{a^3}(1 - e \cos \psi) \sin \psi d\psi}{\sqrt{1 - e \cos \psi - \frac{1 - 2e \cos \psi + e^2 \cos^2 \psi}{2} - \frac{1 - e^2}{2}}} \\
&= \sqrt{\frac{ma^3}{2\kappa}} \int_0^\psi \frac{e(1 - e \cos \psi) \sin \psi d\psi}{\sqrt{1 - e \cos \psi - \frac{1}{2} + e \cos \psi - \frac{e^2 \cos^2 \psi}{2} - \frac{1}{2} + \frac{e^2}{2}}} \\
&= \sqrt{\frac{ma^3}{2\kappa}} \int_0^\psi \frac{e(1 - e \cos \psi) \sin \psi d\psi}{\sqrt{\frac{e^2}{2} - \frac{e^2 \cos^2 \psi}{2}}} \\
&= \sqrt{\frac{ma^3}{2\kappa}} \int_0^\psi \frac{\sqrt{2}(1 - e \cos \psi) \sin \psi d\psi}{\sqrt{(1 - \cos^2 \psi)}} \\
&= \sqrt{\frac{ma^3}{\kappa}} \int_0^\psi \frac{(1 - e \cos \psi) \sin \psi d\psi}{\sin \psi} \\
&= \sqrt{\frac{ma^3}{\kappa}} \int_0^\psi (1 - e \cos \psi) d\psi \\
&= \sqrt{\frac{ma^3}{\kappa}} (\psi - e \sin \psi)
\end{aligned}$$

Therefore naming $\omega = \sqrt{\kappa/ma^3}$ we get that

$$\omega t = \psi - e \sin \psi$$

□

Solution. Exercise 1.7.1 Let a circular orbit such that $r = r_0$ then energy of the system is

$$E_0 = \frac{1}{2}m\dot{r}^2 + V_{\text{eff}}(r)$$

But since r is constant then we have that $\dot{r} = 0$ and hence

$$E_0 = V_{\text{eff}}(r_0)$$

Then taking the time derivative we get that $V'_{\text{eff}}(r_0) = 0$ since E_0 is constant. But also we know that $V_{\text{eff}}(r) = l^2/2mr^2 + V(r)$ hence taking the derivative and making it equal to 0 we get that

$$-\frac{l^2}{mr^3} + V'(r) = 0$$

or replacing $r = r_0$ we get that $V'(r_0) = l^2/mr_0^3$.

Finally, taking the second derivative of $V_{\text{eff}}(r)$ we get that

$$V''_{\text{eff}}(r_0) = \frac{3l^2}{mr_0^4} + V''(r_0) = \frac{3}{r_0} \frac{l^2}{mr_0^3} + V''(r_0) = \frac{3}{r_0} V'(r_0) + V''(r_0)$$

□

Solution. Exercise 1.7.2

- (1) Let $0 < e < 1$, the equation for r is

$$r = \frac{l^2}{m\kappa} \frac{1}{(1 + e \cos \phi)}$$

Then the maximum and minimum of r happen for $\phi = \pi$ and $\phi = 0$ respectively. For $\phi = \pi$ we have that $\cos \pi = -1$ and hence

$$r_{\max} = \frac{l^2}{m\kappa} \frac{1}{1 - e} = p(1 - e)^{-1}$$

And for $\phi = 0$ we get that $\cos 0 = 1$ so

$$r_{\min} = \frac{l^2}{m\kappa} \frac{1}{1 + e} = p(1 + e)^{-1}$$

Where $p = l^2/m\kappa$. Also, since the semi-major axis of an ellipse is given by $a = (r_{\max} + r_{\min})/2$ we get that

$$a = \frac{p(1 - e)^{-1} + p(1 + e)^{-1}}{2} = p \frac{1 + e + 1 - e}{2(1 - e)(1 + e)} = p(1 - e^2)^{-1}$$

- (2) We know that $dA = \frac{1}{2}r^2 d\phi$ then dividing by dt

$$\frac{dA}{dt} = \frac{1}{2}r^2 \frac{d\phi}{dt}$$

But we know that $l = mr^2\dot{\phi}$ then

$$\frac{dA}{dt} = \frac{1}{2m}mr^2 \frac{d\phi}{dt} = \frac{l}{2m}$$

Which is Kepler's second law.

- (3) From Kepler's second law we know that $dA = (l/2m)dt$ so by integration we get that

$$\begin{aligned} \frac{l}{2m} \int_0^\tau dt &= \int_0^A dA \\ \tau &= \frac{2m}{l} A \end{aligned}$$

Replacing $A = \pi ab$ and $b = a\sqrt{1 - e^2}$ we get that

$$\tau = \frac{2m}{l} \pi ab = \frac{2\pi ma^2}{l} \sqrt{1 - e^2}$$

Also from $a = p(1 - e^2)^{-1}$ we know that $1 - e^2 = p/a$ hence

$$\tau = \frac{2\pi ma^2}{l} \sqrt{\frac{p}{a}} = \frac{2\pi ma^2}{l} \sqrt{\frac{l^2}{m\kappa a}} = \frac{2\pi a^2}{\sqrt{a}} \sqrt{\frac{m}{\kappa}} = 2\pi a^{3/2} \sqrt{\frac{m}{\kappa}}$$

□